changed p256_add

code/experimental/P256/Hacl.Impl.P256.fst
@@ -32,6 +32,35 @@ let basepoint_list : x:list uint64 =
 
   l
 
+val add_carry: cin: uint64 -> x: uint64 -> y: uint64 -> result1: lbuffer uint64 (size 1) -> 
+  Stack uint64 
+    (requires fun h -> live h result1)
+    (ensures fun h0 _ h1 -> True)
+
+let add_carry cin x y result1 = 
+  let res1 = x +. cin in 
+  let c = if lt_u64 res1 cin then u64 1 else u64 0 in
+  let res = res1 +. y in
+  let c = if lt_u64 res res1 then c +. u64 1 else c in
+  Lib.Buffer.upd result1 (size 0) res;
+  c
+  
+val sub_borrow: cin: uint64 -> x: uint64 -> y: uint64 -> result1: lbuffer uint64 (size 1) -> 
+  Stack uint64
+    (requires fun h -> live h result1)
+    (ensures fun h0 _ h1 -> True)
+
+let sub_borrow cin x y result1 = 
+  let open Hacl.Spec.Curve25519.Field64.Core in 
+  let res = x -. y -. cin in
+  let c =
+    if eq_u64 cin (u64 1) then
+      (if le_u64 x y then u64 1 else u64 0)
+    else
+      (if lt_u64 x y then u64 1 else u64 0) in
+  Lib.Buffer.upd result1 (size 0) res;
+  c
+
 
 
 #set-options "--z3rlimit 500" 
@@ -47,26 +76,39 @@ val p256_add: arg1: felem -> arg2: felem ->  out: felem -> Stack unit
   )
 
 let p256_add arg1 arg2 out = 
+    push_frame();
   let h0 = ST.get() in 
 
-  let arg1_0 = index arg1 (size 0) in 
-  let arg1_1 = index arg1 (size 1) in 
-  let arg1_2 = index arg1 (size 2) in 
-  let arg1_3 = index arg1 (size 3) in 
+  let a0 = index arg1 (size 0) in 
+  let a1 = index arg1 (size 1) in 
+  let a2 = index arg1 (size 2) in 
+  let a3 = index arg1 (size 3) in 
 
-  let arg2_0 = index arg2 (size 0) in 
-  let arg2_1 = index arg2 (size 1) in 
-  let arg2_2 = index arg2 (size 2) in 
-  let arg2_3 = index arg2 (size 3) in 
+  let b0 = index arg2 (size 0) in 
+  let b1 = index arg2 (size 1) in 
+  let b2 = index arg2 (size 2) in 
+  let b3 = index arg2 (size 3) in 
 
-  let (r0, r1, r2, r3) = felem_add (arg1_0, arg1_1, arg1_2, arg1_3) (arg2_0, arg2_1, arg2_2, arg2_3) in   
+  let r0 = sub out (size 0) (size 1) in 
+  let r1 = sub out (size 1) (size 1) in 
+  let r2 = sub out (size 2) (size 1) in 
+  let r3 = sub out (size 3) (size 1) in 
   
-  upd out (size 0) r0;
-  upd out (size 1) r1;
-  upd out (size 2) r2;
-  upd out (size 3) r3;
+  let cc = add_carry (u64 0) a0 b0 r0 in 
+  let cc = add_carry cc a1 b1 r1 in 
+  let cc = add_carry cc a2 b2 r2 in 
+  let cc = add_carry cc a3 b3 r3 in 
+
+  let t = cc in 
+  let cc = add_carry cc (index r0 (size 0)) (u64 0) r0 in 
+  let cc = add_carry cc (index r1 (size 0)) ((u64 0) -. (t <<. (size 32))) r1 in 
+  let cc = add_carry cc (index r2 (size 0)) ((u64 0) -. t) r2 in 
+  let cc = add_carry cc (index r3 (size 0)) ((t <<. (size 32)) -. (t <<. (size 1))) r3 in 
+
 
   let h1 = ST.get() in 
+  pop_frame();
+  admit();
   assert(Lib.Sequence.equal (as_seq h1 out) (felem_add_seq (as_seq h0 arg1) (as_seq h0 arg2)));
   ()
 
